src/CLI/Analyse_Dispatch.thy
@@ -1040,7 +1040,6 @@ code_identifier
 | code_module Check_Report \<rightharpoonup> (OCaml) Core
 | code_module Contextual_Check_Report \<rightharpoonup> (OCaml) Core
 | code_module Analysis_Result \<rightharpoonup> (OCaml) Core
-| code_module Exec_DG_Bridge \<rightharpoonup> (OCaml) Core
 | code_module Monovariant_Analysis_Result \<rightharpoonup> (OCaml) Core
 | code_module DG_Base_Exec \<rightharpoonup> (OCaml) Core
 | code_module Sign_Arithmetic \<rightharpoonup> (OCaml) Core
